

# Kalman Filter

---

Juan F. Rubio-Ramírez

Emory University

# State Space Form

- Transition equation:

$$x_{t+1} = Fx_t + G\omega_{t+1}, \omega_{t+1} \sim N(0, Q)$$

- Measurement equation

$$z_t = H'x_t + v_t, v_t \sim N(0, R)$$

- Where  $x_t$  are the states and  $z_t$  are the observables
- Assume we want to write the likelihood function of  $z^T = \{z_t\}_{t=1}^T$ .
- A necessary and sufficient condition for the system to be stable is that:

$$|\lambda_i(F)| < 1$$

for all  $i$ , where  $\lambda_i(F)$  stands for eigenvalue of  $F$ .

# The State Space Representation is Not Unique

- Let the following system
  - Transition equation

$$x_{t+1} = Fx_t + G\omega_{t+1}, \omega_{t+1} \sim N(0, Q)$$

- Measurement equation

$$z_t = H'x_t + v_t, v_t \sim N(0, R)$$

- Let  $B$  be a non-singular squared matrix conforming with  $F$ . Then, if  $x_t^* = Bx_t$ ,  $F^* = BFB^{-1}$ ,  $G^* = BG$ , and  $H^* = (H'B)'$ , we can write:

- Transition equation

$$x_{t+1}^* = F^*x_t^* + G^*\omega_{t+1}, \omega_{t+1} \sim N(0, Q)$$

- Measurement equation

$$z_t = H^{*'}x_t^* + v_t, v_t \sim N(0, R)$$

## Example

- Assume the following AR(2) process  $z_t = \rho_1 z_{t-1} + \rho_2 z_{t-2} + v_t$ ,  $v_t \sim N(0, \sigma_v^2)$ .
- State Space I

- Transition equation

$$x_t = \begin{bmatrix} \rho_1 & 1 \\ \rho_2 & 0 \end{bmatrix} x_{t-1} + \begin{bmatrix} 1 \\ 0 \end{bmatrix} v_t$$

- Where  $x_t = \begin{bmatrix} y_t & \rho_2 y_{t-1} \end{bmatrix}'$  and measurement equation  $z_t = \begin{bmatrix} 1 & 0 \end{bmatrix} x_t$

- State Space II

- Transition equation

$$x_t = \begin{bmatrix} \rho_1 & \rho_2 \\ 1 & 0 \end{bmatrix} x_{t-1} + \begin{bmatrix} 1 \\ 0 \end{bmatrix} v_t$$

- Where  $x_t = \begin{bmatrix} y_t & y_{t-1} \end{bmatrix}'$  and measurement equation  $z_t = \begin{bmatrix} 1 & 0 \end{bmatrix} x_t$

- Try  $B = \text{diag} \begin{pmatrix} 1 & \rho_2 \end{pmatrix}$  on the second system to get the first system.

# What is the Kalman Filter trying to do?

- Let  $x_{t|t-1} = E(x_t|z^{t-1})$ .
- Let  $z_{t|t-1} = E(z_t|z^{t-1}) = H'x_{t|t-1}$ .
- Let  $x_{t|t} = E(x_t|z^t)$ .
- Let assume we have  $x_{t|t-1}$  and  $z_{t|t-1}$ .
- We observe a new  $z_t$ .
- We need to obtain  $x_{t|t}$ .
- Note that  $x_{t+1|t} = Fx_{t|t}$  and  $z_{t+1|t} = H'x_{t+1|t}$ , so we can wait for  $z_{t+1}$ .
- Therefore, the key question is how to obtain from  $x_{t|t-1}$  and  $z_t$ .

## Kalman Filter Gain to find $x_{t|t}$

- Assume we use the following equation to get  $x_{t|t}$  from  $z_t$  and  $x_{t|t-1}$ :

$$x_{t|t} = x_{t|t-1} + K_t (z_t - z_{t|t-1}) = x_{t|t-1} + K_t (z_t - H'x_{t|t-1})$$

- This formula will have some probabilistic justification (to follow).
- $K_t$  is called the Kalman filter gain and it measures how much we update  $x_{t|t-1}$  as a function in our error in predicting  $z_t$ .
- Let  $\Sigma_{t|t-1} = E \left( (x_t - x_{t|t-1}) (x_t - x_{t|t-1})' | z^{t-1} \right)$ .
- Let  $\Omega_{t|t-1} = E \left( (z_t - z_{t|t-1}) (z_t - z_{t|t-1})' | z^{t-1} \right)$ .
- Let  $\Sigma_{t|t} = E \left( (x_t - x_{t|t}) (x_t - x_{t|t})' | z^t \right)$ .
- Let  $\Phi_{t|t-1} = E \left( (z_t - z_{t|t}) (x_t - x_{t|t})' | z^{t-1} \right)$ .
- It can be shown that:

$$K_t = \Sigma_{t|t-1} H (H' \Sigma_{t|t-1} H + R)^{-1}$$

- The gain:

$$K_t = \Sigma_{t|t-1} H (H' \Sigma_{t|t-1} H + R)^{-1}$$

- Update of  $x_{t|t}$  given  $z_t$  and  $x_{t|t-1}$  being:

$$x_{t|t} = x_{t|t-1} + K_t (z_t - H' x_{t|t-1})$$

- If we did a big mistake forecasting  $x_{t|t-1}$  using past information ( $\Sigma_{t|t-1}$  large) we give a lot of weight to the new information ( $K_t$  large).
- If the new information is noise ( $R$  large) we give a lot of weight to the old prediction ( $K_t$  small)

## Example

- Assume the following model in State Space form:

- Transition equation

$$x_t = \mu + v_t, v_t \sim N(0, \sigma_v^2)$$

- Measurement equation

$$z_t = x_t + \xi_t, \xi_t \sim N(0, \sigma_\xi^2)$$

- Let  $\sigma_\xi^2 = q\sigma_v^2$ .

- Then, if  $\Sigma_{t|t-1} = \sigma_v^2$ , we have

$$K_t = \sigma_v^2 \frac{1}{1+q} \propto \frac{1}{1+q}.$$

- The bigger  $\sigma_\xi^2$  relative to  $\sigma_v^2$  (the bigger  $q$ ) the lower  $K_t$  and the less we trust  $z_t$ .



# The Algorithm

- Given  $\Sigma_{t|t-1}$ ,  $z_t$ , and  $x_{t|t-1}$ , we can now set the Kalman filter algorithm:
- Let  $\Sigma_{t|t-1}$ , then we compute:  $\Omega_{t|t-1} = E \left( (z_t - z_{t|t-1}) (z_t - z_{t|t-1})' | z^{t-1} \right)$   
$$= E \left( \begin{array}{c} H' (x_t - x_{t|t-1}) (x_t - x_{t|t-1})' H + \\ v_t (x_t - x_{t|t-1})' H + H' (x_t - x_{t|t-1}) v_t' + \\ v_t v_t' | z^{t-1} \end{array} \right) = H' \Sigma_{t|t-1} H + R$$
- Let  $\Sigma_{t|t-1}$ , then we compute:  $\Phi_{t|t-1} = E \left( (z_t - z_{t|t-1}) (x_t - x_{t|t-1})' | z^{t-1} \right)$   
$$= E \left( H' (x_t - x_{t|t-1}) (x_t - x_{t|t-1})' + v_t (x_t - x_{t|t-1})' | z^{t-1} \right) = H' \Sigma_{t|t-1}$$
- Let  $\Sigma_{t|t-1}$ , then we compute  $K_t = \Sigma_{t|t-1} H (H' \Sigma_{t|t-1} H + R)^{-1}$ .
- Let  $\Sigma_{t|t-1}$ ,  $x_{t|t-1}$ ,  $K_t$ , and  $z_t$  then we compute  $x_{t|t} = x_{t|t-1} + K_t (z_t - H' x_{t|t-1})$

# The Algorithm

- Let  $\Sigma_{t|t-1}$  and  $K_t$ , then we compute:  $\Sigma_{t|t} = E \left( (x_t - x_{t|t}) (x_t - x_{t|t})' | z^t \right)$   
$$= E \left( \begin{array}{c} (x_t - x_{t|t-1}) (x_t - x_{t|t-1})' - \\ (x_t - x_{t|t-1}) (z_t - H'x_{t|t-1})' K_t' - \\ K_t (z_t - H'x_{t|t-1}) (x_t - x_{t|t-1})' + \\ K_t (z_t - H'x_{t|t-1}) (z_t - H'x_{t|t-1})' K_t' | z^t \end{array} \right) = \Sigma_{t|t-1} - K_t H' \Sigma_{t|t-1}$$
- Let  $\Sigma_{t|t}$ , then we compute  $\Sigma_{t+1|t} = F \Sigma_{t|t} F' + G Q G'$
- Let  $x_{t|t}$ , then we compute:
  - $x_{t+1|t} = F x_{t|t}$
  - $z_{t+1|t} = H' x_{t+1|t}$
- Therefore, from  $x_{t|t-1}$ ,  $\Sigma_{t|t-1}$ , and  $z_t$  we compute  $x_{t|t}$  and  $\Sigma_{t|t}$ .
- We also compute  $z_{t|t-1}$ ,  $\Omega_{t|t-1}$ , and  $\Phi_{t|t-1}$ . Why for? As you will see later, they are necessary to calculate the likelihood function of  $z^T = \{z_t\}_{t=1}^T$  (to follow).

We start with  $x_{t|t-1}$  and  $\Sigma_{t|t-1}$ , then we observe  $z_t$  and....

- $\Omega_{t|t-1} = H'\Sigma_{t|t-1}H + R$
- $z_{t|t-1} = H'x_{t|t-1}$
- $K_t = \Sigma_{t|t-1}H (H'\Sigma_{t|t-1}H + R)^{-1}$
- $\Sigma_{t|t} = \Sigma_{t|t-1} - K_t H' \Sigma_{t|t-1}$
- $x_{t|t} = x_{t|t-1} + K_t (z_t - H'x_{t|t-1})$
- $\Sigma_{t+1|t} = F\Sigma_{t|t}F' + GQG'$
- $x_{t+1|t} = Fx_{t|t}$

We finish with  $x_{t+1|t}$  and  $\Sigma_{t+1|t}$ .

## A Probabilistic Approach to $K_t$

- Assume

$$Z|w = [X'|w \ Y'|w]' \sim N \left( \begin{bmatrix} \bar{x} \\ \bar{y} \end{bmatrix}, \begin{bmatrix} \Sigma_{xx} & \Sigma_{xy} \\ \Sigma_{yx} & \Sigma_{yy} \end{bmatrix} \right)$$

- then

$$X|y, w \sim N \left( \bar{x} + \Sigma_{xy} \Sigma_{yy}^{-1} (y - \bar{y}), \Sigma_{xx} - \Sigma_{xy} \Sigma_{yy}^{-1} \Sigma_{yx} \right)$$

- But  $x_{t|t-1} = E(x_t|z^{t-1})$  and  $\Sigma_{t|t-1} = E((x_t - x_{t|t-1})(x_t - x_{t|t-1})' | z^{t-1})$
- If  $z_t|z^{t-1}$  is the random variable  $z_t$  (observable) conditional on  $z^{t-1}$ , then:
  - Let  $z_{t|t-1} = H'x_{t|t-1}$
  - Let  $\Omega_{t|t-1} = H'\Sigma_{t|t-1}H + R$
  - Let  $\Phi_{t|t-1} = H'\Sigma_{t|t-1}$

## A Probabilistic Approach to $K_t$

- Assume we know  $x_{t|t-1}$  and  $\Sigma_{t|t-1}$ , then

$$\begin{pmatrix} x_t \\ z_t \end{pmatrix} | z^{t-1} \sim N \left( \begin{bmatrix} x_{t|t-1} \\ H' x_{t|t-1} \end{bmatrix}, \begin{bmatrix} \Sigma_{t|t-1} & \Sigma_{t|t-1} H \\ H' \Sigma_{t|t-1} & H' \Sigma_{t|t-1} H + R \end{bmatrix} \right)$$

- Remember that:

$$X|y, w \sim N \left( \bar{x} + \Sigma_{xy} \Sigma_{yy}^{-1} (y - \bar{y}), \Sigma_{xx} - \Sigma_{xy} \Sigma_{yy}^{-1} \Sigma_{yx} \right)$$

- Then, we can write  $x_t | z_t, z^{t-1} = x_t | z^t \sim N(x_{t|t}, \Sigma_{t|t})$ , where

$$x_{t|t} = x_{t|t-1} + \underbrace{\Sigma_{t|t-1} H (H' \Sigma_{t|t-1} H + R)^{-1}}_{K_t} (z_t - H' x_{t|t-1})$$

$$\Sigma_{t|t} = \Sigma_{t|t-1} - \underbrace{\Sigma_{t|t-1} H (H' \Sigma_{t|t-1} H + R)^{-1} H' \Sigma_{t|t-1}}_{K_t}$$